Work in progress

src/TupleEnsembles.v
@@ -8,6 +8,47 @@ Require Import
 
 Generalizable All Variables.
 
+Definition Map_set {A B} (f : A -> B) (r : Ensemble A) : Ensemble B :=
+  fun b => exists a : A, In _ r a /\ b = f a.
+
+Lemma Map_set_left_identity {A} (r : Ensemble A) : Same_set A r (Map_set id r).
+Proof.
+  unfold Map_set; split; intros.
+    eexists; intuition.
+    assumption.
+  intros ??.
+  do 2 destruct H.
+  unfold id in H0.
+  congruence.
+Qed.
+
+Lemma Map_set_right_identity {A} (r : Ensemble A) : Same_set A (Map_set id r) r.
+Proof.
+  unfold Map_set; split; intros.
+    intros ??.
+    do 2 destruct H.
+    unfold id in H0.
+    congruence.
+  eexists; intuition.
+  assumption.
+Qed.
+
+Lemma Map_set_composition {A B C} (r : Ensemble A) :
+  forall (f : B -> C) (g : A -> B),
+   Same_set C (Map_set (fun x => f (g x)) r) (Map_set f (Map_set g r)).
+Proof.
+  unfold Map_set; split; intros; intros ??.
+    do 2 destruct H; subst.
+    exists (g x0); simpl in *.
+    split; trivial.
+    exists x0; simpl.
+    intuition.
+  do 2 destruct H; subst.
+  do 2 destruct H; simpl in *; subst.
+  exists x; simpl in *.
+  intuition.
+Qed.
+
 Section TupleEnsemble.
 
 Variables A B : Type.
@@ -154,11 +195,18 @@ Definition Modify (a : A) (f : B -> B) (r : Ensemble (A * B)) :
      P  = ((2, Some 3), (3, Some 2))
    Then [Overlay P r' r] would be [((1,6), (2,11), (3,10))]. *)
 
-Definition Overlay (P : A -> option A) (r' r : Ensemble (A * B)) :
+(*
+Definition Overlay (b1 b2 : N) (r r' : Ensemble (A * B)) :
   Ensemble (A * B) :=
   Ensembles.Union
-    _ (Relate (fun k e k' e' => P k' = Some k /\ e = e') r)
+    _ (ContraMap_set
+         (fun p => match P (fst p) with
+                   | Some k => (k, snd p)
+                   | None => p
+                   end)
+         (Filter (fun k _ => exists k', P k' = Some k) r))
       (Filter (fun k _ => P k = None) r').
+*)
 
 Definition All (P : A -> B -> Prop) (r : Ensemble (A * B)) : Prop :=
   forall a b, Lookup a b r -> P a b.
@@ -356,6 +404,7 @@ Proof.
   firstorder.
 Qed.
 
+(*
 Lemma Lookup_Overlay : forall a b P r' r,
   match P a with
   | Some a' => Lookup a' b r
@@ -366,6 +415,7 @@ Proof.
   apply Lookup_Union.
   destruct (P a) eqn:Heqe.
     left.
+(*
     eapply Lookup_Relate.
       exact H.
     intuition.
@@ -373,6 +423,8 @@ Proof.
   apply Lookup_Filter.
   intuition.
 Qed.
+*)
+Admitted.
 
 Lemma Lookup_Overlay_inv : forall a b P r' r,
   Lookup a b (Overlay P r' r)
@@ -384,6 +436,7 @@ Proof.
   unfold Overlay; intros.
   apply Lookup_Union_inv in H.
   destruct H.
+(*
     apply Lookup_Relate_inv in H.
     do 4 destruct H; subst.
     rewrite H; assumption.
@@ -391,6 +444,9 @@ Proof.
   destruct H.
   rewrite H; assumption.
 Qed.
+*)
+Admitted.
+*)
 
 Lemma Lookup_Member : forall a b r,
   Lookup a b r -> Member a r.
@@ -435,7 +491,9 @@ Arguments Relate : default implicits.
 Arguments All : default implicits.
 Arguments Any : default implicits.
 Arguments Define : default implicits.
+(*
 Arguments Overlay : default implicits.
+*)
 Arguments Lookup : default implicits.
 Arguments Same : default implicits.
 Arguments Member : default implicits.
@@ -488,7 +546,7 @@ Ltac teardown :=
   | [ H : Lookup _ _ (Filter _ _)    |- _ ] => apply Lookup_Filter_inv in H
   | [ H : Lookup _ _ (Define _ _ _)  |- _ ] => apply Lookup_Define_inv in H
   | [ H : Lookup _ _ (Modify _ _ _)  |- _ ] => apply Lookup_Modify_inv in H
-  | [ H : Lookup _ _ (Overlay _ _ _) |- _ ] => apply Lookup_Overlay_inv in H
+  (* | [ H : Lookup _ _ (Overlay _ _ _) |- _ ] => apply Lookup_Overlay_inv in H *)
   | [ H : Lookup _ _ (Union _ _ _)   |- _ ] => apply Lookup_Union_inv in H
 
   | [ H : Member _ Empty           |- _ ] => unfold Member in H
@@ -502,7 +560,8 @@ Ltac teardown :=
   | [ H : Member _ (Filter _ _)    |- _ ] => unfold Member in H
   | [ H : Member _ (Define _ _ _)  |- _ ] => unfold Member in H
   | [ H : Member _ (Modify _ _ _)  |- _ ] => unfold Member in H
-  | [ H : Member _ (Overlay _ _ _) |- _ ] => unfold Member in H
+  (* | [ H : Member _ (Overlay _ _ _) |- _ ] => unfold Member in H *)
+  | [ H : Member _ (Union _ _ _)   |- _ ] => unfold Member in H
 
   | [ |- Lookup _ _ Empty           ] => apply Lookup_Empty
   | [ |- Lookup _ _ (Single _ _)    ] => apply Lookup_Single
@@ -515,7 +574,7 @@ Ltac teardown :=
   | [ |- Lookup _ _ (Filter _ _)    ] => apply Lookup_Filter
   | [ |- Lookup _ _ (Define _ _ _)  ] => apply Lookup_Define
   | [ |- Lookup _ _ (Modify _ _ _)  ] => apply Lookup_Modify
-  | [ |- Lookup _ _ (Overlay _ _ _) ] => apply Lookup_Overlay
+  (* | [ |- Lookup _ _ (Overlay _ _ _) ] => apply Lookup_Overlay *)
   | [ |- Lookup _ _ (Union _ _ _)   ] => apply Lookup_Union
 
   | [ H : Lookup ?X ?Y ?R |- Member ?X ?R ] => exists Y; exact H
